The polynomial $\polynomialP{m}{b}{x}, \; m\in\mathbb{N}$ is $2m+1$-degree integer-valued polynomial in $x,b\in\mathbb{R}$.
\[
    \polynomialP{m}{b}{x} = \sum_{k=0}^{b-1} \sum_{r=0}^{m} \coeffA{m}{r} k^r(x-k)^r,
\]
where $\coeffA{m}{r}$ is real coefficient.
By means of Lemma~\ref{lemma_polynomial_p_and_odd_power},
the polynomial $\polynomialP{m}{b}{x}$ has the following relation with Binomial theorem~\cite{AbraSteg72}
\[
    \polynomialP{m}{x+y}{x+y} = \sum_{r=0}^{2m+1} \binom{2m+1}{r} x^{2m+1-r} y^r.
\]
From the other hand, polynomial $\polynomialP{m}{b}{x}$ might be expressed in terms of discrete convolution
of polynomial $n^j, \; j\in \mathbb{N}$
\[
    \polynomialP{m}{x+1}{x} = \sum_{r=0}^{m} \coeffA{m}{r} \convPower{n}{r}{x}, \quad n\geq 0.
\]
Therefore, it is easy to notice the following identities in terms of Binomial theorem and discrete convolution,
see Corollaries~\ref{cor_bin_exp_and_macaulay_conv},~\ref{cor_bin_exp_and_macaulay_conv_strict}
\begin{equation*}
    \sum_{r=0}^{m} \coeffA{m}{r} \convPower{n}{r}{x+y}
    =
    1 + \sum_{r=0}^{2m+1} \binom{2m+1}{r} x^{2m+1-r} y^r, \quad n \geq 0.
\end{equation*}
\begin{equation*}
    \sum_{r=0}^{m} \coeffA{m}{r} \convPower{n}{r}{x+y}
    =
    -1 + \sum_{r=0}^{2m+1} \binom{2m+1}{r} x^{2m+1-r} y^r, \quad n \geq 1.
\end{equation*}
Also, the following generalizations for multinomial case are discussed,
see Corollaries~\ref{cor_mult_exp_and_macaulay_conv},~\ref{cor_mult_exp_and_macaulay_conv_strict}
\begin{gather*}
    \sum_{r=0}^{m} \coeffA{m}{r} \convPower{n}{r}{\multifoldSum{t}} =
    1 + \sum_{\multifoldSum[k]{t}=2m+1} \binom{2m+1}{k_1, k_2,\ldots, k_t} \prod_{\ell=1}^{t} x_\ell^{k_\ell},
    \quad n \geq 0.\\
    \sum_{r=0}^{m} \coeffA{m}{r} \convPower{n}{r}{\multifoldSum{t}} =
    -1 + \sum_{\multifoldSum[k]{t}=2m+1} \binom{2m+1}{k_1, k_2,\ldots, k_t} \prod_{\ell=1}^{t} x_\ell^{k_\ell},
    \quad n \geq 1.\\
\end{gather*}
A few polynomial identities are straightforward as well,
Theorems~\ref{thm_odd_power_by_macaulays_convolution},~\ref{thm_odd_power_by_macaulays_convolution_strict}
\begin{gather*}
    x^{2m+1} = \sum_{r=0}^{m} \coeffA{m}{r} \sum_{k=0}^{x-1} k^r (x-k)^r,\\
    x^{2m+1} = \sum_{r=0}^{m} \coeffA{m}{r} \sum_{k=1}^{x} k^r (x-k)^r.\\
\end{gather*}