\begin{lem}
    \label{lemma_polynomial_p_and_odd_power}
    For every $m\in\mathbb{N}, \; x,y\in\mathbb{R}$
    \begin{equation*}
        \polynomialP{m}{x+y}{x+y} = \sum_{r=0}^{2m+1} \binom{2m+1}{r} x^{2m+1-r} y^r
    \end{equation*}
\end{lem}
By Lemma~\ref{lemma_polynomial_p_and_odd_power} and equation~\eqref{eq:p_all_forms} the following
polynomial identities straightforward
\begin{equation*}
    x^{2m+1}
    =\sum_{r=0}^{m} \sum_{\ell=1}^{2m-r+1} (-1)^{2m-r} \coeffH{m}{r}{\ell} \cdot x^{\ell+r}
    =\sum_{r=0}^{m} (-1)^{m-r} \polynomialX{m}{r}{x} \cdot x^r
\end{equation*}
For instance,
\begin{equation*}
    \polynomialP{2}{x+y}{x+y} = (x + y) (x^4 + 4 x^3 y + 6 x^2 y^2 + 4 x y^3 + y^4).
\end{equation*}
In addition, the following identities hold
\begin{equation*}
    \begin{split}
    (x+y)
        ^{2m+1}
        &=\sum_{r=0}^{m} \sum_{\ell=1}^{2m-r+1} (-1)^{2m-r} \coeffH{m}{r}{\ell} \cdot (x+y)^{\ell+r} \\
        &=\sum_{r=0}^{m} (-1)^{m-r} \polynomialX{m}{r}{x+y} \cdot (x+y)^r
    \end{split}
\end{equation*}
Obviously, Multinomial expansion of $t$-fold sum $(\multifoldSum{t})^{2m+1}$ can be reached
by $\polynomialP{m}{b}{\multifoldSum{t}}$ as well
\begin{cor}
    For all $x_1,x_2,\ldots, x_t\in\mathbb{R}, \; m \in \mathbb{N}$
    \begin{equation*}
        \polynomialP{m}{\multifoldSum{t}}{\multifoldSum{t}}
        =
        \sum_{\multifoldSum[k]{t}=2m+1} \binom{2m+1}{k_1, k_2,\ldots, k_t} \prod_{s=1}^{t} x_t^{k_s}
    \end{equation*}
\end{cor}
Moreover, the following multinomial identities hold
\begin{equation*}
    \begin{split}
    (\multifoldSum{t})
        ^{2m+1}
        &=\sum_{r=0}^{m} \sum_{\ell=1}^{2m-r+1} (-1)^{2m-r} \coeffH{m}{r}{\ell} \cdot (\multifoldSum{t})^{\ell+r} \\
        &=\sum_{r=0}^{m} (-1)^{m-r} \polynomialX{m}{r}{\multifoldSum{t}} \cdot (\multifoldSum{t})^r
    \end{split}
\end{equation*}
